Fix linear search study cases

caseStudy/linearSearchAT.dfy
@@ -6,11 +6,11 @@ import opened SumReal
 import opened TypeR0
 import opened ComplexityR0
 
-ghost predicate inv<A>(s:seq<A>, x:A, i:nat, N:int)
+ghost predicate inv<A>(s:seq<A>, x:A, i:nat, n:nat)
 {
-     0 <= i <= N && N <= |s|
-  && (0 <= N < |s| ==> s[i] == x)      
-  && (N == |s|     ==> (forall j :: 0 <= j < i ==> s[j] != x))
+     0 <= i <= n && n <= |s|
+  && (0 <= n < |s| ==> s[i] == x)      
+  && (n == |s|     ==> (forall j :: 0 <= j < i ==> s[j] != x))
 }
 
 ghost predicate post<A>(s:seq<A>, x:A, i:nat)
@@ -33,14 +33,14 @@ ghost method linearSearch<A>(s:seq<A>, x:A) returns (i:nat, t:nat)
   ensures  post(s, x, i)
   ensures  exists k :: 0 <= k < |s| && s[k] == x && t == T(s, x, k)
 {
-  var N;
-  i, N, t := 0, |s|, 1;
-  while i != N && s[i] != x
-    invariant inv(s, x, i, N)
+  var n:nat;
+  i, n, t := 0, |s|, 1;
+  while i != n && s[i] != x
+    invariant inv(s, x, i, n)
     invariant forall j :: 0 <= j < i ==> s[j] != x
     invariant exists k :: i <= k < |s| && s[k] == x
     invariant t == i+1
-    decreases N - i
+    decreases n - i
   {
     i := i + 1;
     t := t + 1;
@@ -56,8 +56,8 @@ ghost function Tavg(N:nat) : R0
 ghost method expectationLoop<A>(N:nat)
   returns (tE:real)
   requires N > 0
-  ensures tE == Tavg(N)
-  ensures tIsBigO(N, tE, n => n as R0)
+  ensures  tE == Tavg(N)
+  ensures  tIsBigO(N, tE, n => n as R0)
 {
   tE := 0.0; 
   var p := 0; reveal sum();  
@@ -85,8 +85,8 @@ ghost method expectationLoop<A>(N:nat)
 
 ghost function probability<A>(s:seq<A>, x:A, p:nat) : R0
   requires 0 <= p < |s|
-  requires forall i, j :: 0 <= i < j < |s| ==> s[i] != s[j]
   requires s[p] == x
+  requires forall i :: 0 <= i < |s| && i != p ==> s[i] != s[p]
 {
   1.0 / |s| as R0
 }
@@ -95,12 +95,12 @@ ghost method inputScenario<A>(N:nat, p:nat) returns (s0:seq<A>, x0:A)
   requires N > 0
   requires 0 <= p < N
   ensures  |s0| == N
-  ensures  forall i, j :: 0 <= i < j < |s0| ==> s0[i] != s0[j]
   ensures  s0[p] == x0
+  ensures  forall i :: 0 <= i < |s0| && i != p ==> s0[i] != s0[p]
 {
   assume {:axiom} 
-    exists s:seq<A> :: |s| == N && (forall i, j :: 0 <= i < j < N ==> s[i] != s[j]);
-  s0 :| |s0| == N && forall i, j :: 0 <= i < j < N ==> s0[i] != s0[j];
+    exists s:seq<A> :: |s| == N && (forall i :: 0 <= i < N && i != p ==> s[i] != s[p]);
+  s0 :| |s0| == N && forall i :: 0 <= i < N && i != p ==> s0[i] != s0[p];
   assume {:axiom} 
     exists x:A :: s0[p] == x;
   x0 :| s0[p] == x0;
