caseStudy/linearSearchBT.dfy
@@ -1,0 +1,109 @@
+include "../theory/math/ExpReal.dfy"
+include "../theory/math/LemFunction.dfy"
+include "../theory/math/SumReal.dfy"
+include "../theory/math/TypeR0.dfy"
+include "../theory/ComplexityNat.dfy"
+
+import opened ExpReal
+import opened LemFunction
+import opened SumReal
+import opened TypeR0
+import opened ComplexityNat
+
+ghost predicate inv<A>(s:seq<A>, x:A, i:nat, n:nat)
+{
+     0 <= i <= n && n <= |s|
+  && (0 <= n < |s| ==> s[i] == x)      
+  && (n == |s|     ==> (forall j :: 0 <= j < i ==> s[j] != x))
+}
+
+ghost predicate post<A>(s:seq<A>, x:A, i:nat)
+{
+     (0 <= i < |s| ==> s[i] == x)
+  && (i == |s|     ==> (forall j :: 0 <= j < |s| ==> s[j] != x))
+}
+
+ghost function f1(N:nat) : nat
+{
+  0
+}
+
+ghost method linearSearchBT1<A>(s:seq<A>, x:A) returns (i:nat, t:nat)
+  ensures post(s, x, i)
+  ensures t == f1(|s|) 
+  ensures tIsBigO(|s|, t, constGrowth())
+{
+  assume {:axiom} |s| == 0;  // best case
+  var n:nat;
+  i, n, t := 0, |s|, 0;
+  while i != n
+    invariant inv(s, x, i, n)
+    invariant i == 0 && t == 0
+    decreases n - i
+  {
+    if s[i] != x {  // Op. interesante
+      i := i+1 ;     
+    } else {
+      n := i;  // break;
+    }
+    t := t + 1;
+  }
+  assert t == f1(|s|);
+  assert bigO(f1, constGrowth()) by { var c, n0 := lem_f1BigOconst(); }
+} 
+
+ghost function f2(N:nat) : nat
+{
+  1
+}
+
+ghost method linearSearchBT2<A>(s:seq<A>, x:A) returns (i:nat, t:nat)
+  ensures post(s, x, i)
+  ensures t == f2(|s|) 
+  ensures tIsBigO(|s|, t, constGrowth())
+{
+  assume {:axiom} |s| > 0 && s[0] == x;  // best case when not empty
+  var n:nat;
+  i, n, t := 0, |s|, 0;
+  while i != n
+    invariant inv(s, x, i, n)
+    invariant i < n  ==> t == 0
+    invariant i == n ==> t == 1
+    decreases n - i
+  {
+    if s[i] != x {  // Op. interesante
+      i := i+1 ;     
+    } else {
+      n := i;  // break;
+    }
+    t := t + 1;
+  }
+  assert t == f2(|s|);
+  assert bigO(f2, constGrowth()) by { var c, n0 := lem_f2BigOconst(); }
+} 
+
+lemma lem_f1BigOconst() returns (c:nat, n0:nat)
+  ensures bigOfrom(c, n0, f1, constGrowth())
+{
+  // we show that c=1 and n0=0
+  c, n0 := 1, 0;
+  forall n:nat | 0 <= n0 <= n
+    ensures f1(n) <= c*constGrowth()(n)
+  {
+    assert f1(n) == 0;
+    assert f1(n) <= c*constGrowth()(n); 
+  }
+}
+
+lemma lem_f2BigOconst() returns (c:nat, n0:nat)
+  ensures bigOfrom(c, n0, f2, constGrowth())
+{
+  // we show that c=1 and n0=0
+  c, n0 := 1, 0;
+  forall n:nat | 0 <= n0 <= n
+    ensures f2(n) <= c*constGrowth()(n)
+  {
+    assert f2(n) == 1;
+    assert f2(n) <= c*constGrowth()(n); 
+  }
+}
